\section{Solving Differential Equations with Laplace Transforms}\label{sec:Solve_Diff_Eqns_Laplace}
\begin{example}[]{Solve Differential Equation with Laplace Transform 1}
  Given the ODE
  \begin{equation*}
    y''(t) + 4y(t) = \delta(t-\pi) \; y(0) = 0, \, y'(0) = 0
  \end{equation*}

  \tcblower

  \begin{align*}
    \Lapl \lbrace y''(t) \rbrace + \Lapl \lbrace 4 y(t) \rbrace &= \Lapl \lbrace \delta (t - \pi) \\
    \left(  -y'(0) - sy(0) + s^{2}Y(s) \right) + 4Y(s) &= e^{-s \pi} \\
    \left( s^{2}Y(s) - 0 - s(0) \right) + 4Y(s) &= e^{-s \pi} \\
    Y(s) \left( s^{2} + 4 \right) &= e^{-s \pi} \\
    Y(s) &= \frac{e^{-s \pi}}{s^{2}+4} \\
    y(t) &= \Lapl^{-1} \biggl\lbrace \frac{e^{-s \pi}}{s^{2}+4} \biggr\rbrace = \biggl\lbrace \frac{e^{-s \pi}}{s^{2}+4} + \frac{0}{s^{2}+4} \biggr\rbrace
  \end{align*}
  Now using our Laplace Transform table we receive our answer.
  \begin{equation*}
    y(t) = 0 + \UnitStep(t - \pi) \frac{1}{2}\sin \left( 2 \left( t - \pi \right) \right)
  \end{equation*}
\end{example}

\begin{example}[]{Solve Differential Equation with Laplace Transform 2}
  Given the ODE
  \begin{equation*}
    y''(t) + 2y'(t) + 2y(t) = \delta (t - \pi) \; y(0) = 1, \, y'(0) = 0
  \end{equation*}

  \tcblower

  \begin{align*}
    \Lapl \lbrace y''(t) \rbrace + \Lapl \lbrace 2y'(t) \rbrace + \Lapl \lbrace 2 y(t) \rbrace &= \Lapl \lbrace \delta (t - \pi) \\
    \Lapl \lbrace y''(t) \rbrace + 2 \Lapl \lbrace y'(t) \rbrace + 2 \Lapl \lbrace y(t) \rbrace &= \Lapl \lbrace \delta (t - \pi) \\
    \left( -y'(0) -sy(0) + s^{2}Y(s) \right) + 2 \left( -y(0) + sY(s) \right) + 2Y(s) &= e^{-s \pi} \\
    \left( -0 - 1s + s^{2}Y(s) \right) + 2 \left( -1 + sY(s) \right) + 2Y(s) &= e^{-s \pi} \\
    \left( -s + s^{2}Y(s) \right) + -2 + 2sY(s) + 2Y(s) &= e^{-s \pi} \\
    s^{2}Y(s) + 2sY(s) + 2Y(s) &= e^{-s \pi} + s + 2 \\
    Y(s) \left( s^{2} + 2s + 2 \right) &= e^{-s \pi} + s + 2 \\
    Y(s) &= \frac{e^{-s \pi} + s + 2}{s^{2} + 2s + 2} \\
    Y(s) &= \frac{e^{-s \pi} + s + 2}{{(s + 1)}^{2} + 1}
  \end{align*}
  Now we perform partial fraction decomposition and receive
  \begin{align*}
    Y(s) &= \frac{e^{-s \pi}}{{(s + 1)}^{2} + 1} + \frac{s+1}{{(s + 1)}^{2} + 1} + \frac{1}{{(s + 1)}^{2} + 1} \\
    y(t) &= \Lapl \Biggl\lbrace \frac{e^{-s \pi}}{{(s + 1)}^{2} + 1} \Biggr\rbrace + \Lapl \Biggl\lbrace \frac{s+1}{{(s + 1)}^{2} + 1} \Biggr\rbrace + \Lapl \Biggl\lbrace \frac{1}{{(s + 1)}^{2} + 1} \Biggr\rbrace
  \end{align*}
  Now, using our handy-dandy Laplace Transform table, we receive our answer.
  \begin{equation*}
    y(t) = \UnitStep(t-\pi)e^{-(t-\pi)}\sin(t-\pi) + e^{-t}\cos(t-\pi) + e^{-t}\sin(t-\pi)
  \end{equation*}
\end{example}

%%% Local Variables:
%%% mode: latex
%%% TeX-master: "../Math_252-Reference_Sheet"
%%% End:
