\section*{Laplace Transform} \label{sec:Laplace Transform}
	\vspace{-2mm}
	\subsection*{Laplace Transform Properties} \label{subsec:Laplace Transform Properties}
		\vspace{-2mm}
		\begin{table}[h!]
			\renewcommand{\arraystretch}{1.4}
			\begin{tabular}{|l|c|c|}
				\hline
				\multicolumn{1}{|c|}{\textbf{Property Name}} & \multicolumn{1}{|c|}{\textbf{Time Domain}}& \multicolumn{1}{|c|}{\textbf{Frequency Domain}} \\ \hline
				Laplace Transform & $x(t) = \frac{1}{2j\pi} \int_{\sigma-\infty}^{\sigma+\infty} X(s) e^{st} ds$ & $X(s) = \int_{0^{-}}^{\infty} x(t) e^{-st} dt$ \\ \hline
				Linearity & $x(t) = \alpha_{1} x_{1}(t) + \alpha_{2} x_{2}(t)$ & $X(s) = \alpha X_{1}(s) + \alpha_{2} X_{2}(s)$ \\ \hline
				Time Scaling & $x(at) \text{, where } a>0$ & $\frac{1}{a} X \left( \frac{s}{a} \right)$ \\ \hline
				Time Shift & $x(t-a) \text{, where } a>0$ & $X(s)e^{-as}$ \\ \hline
				Frequency Shift & $x(t)e^{at}$ & $X(s)(s-a)$ \\ \hline
				Multiplication by $\sin \left( \omega_{0} t \right)$ & $x(t) \sin \left( \omega_{0} t \right)$ & $\frac{j}{2} \left[  X(s+j\omega_{0}) - X(s-j\omega_{0}) \right]$ \\ \hline
				Multiplication by $\cos \left( \omega_{0} t \right)$ & $x(t) \cos \left( \omega_{0} t \right)$ & $\frac{j}{2} \left[  X(s+j\omega_{0}) + X(s-j\omega_{0}) \right]$ \\ \hline
				Multiply by t in Time, Derivative in Frequency & $t^{n} x(t)$ & $(-1)^{n} \frac{d^{n}}{ds^{n}} X(s)$ \\ \hline
				Mutliply by s in Frequency, Derivative in Time & $\frac{d^{n}}{dt^{n}} x(t)$ & $s^{n}X(s) - \sum_{i=0}^{n-1} s^{n-1-i} \frac{d^{i}}{dt^{i}} x(t) \vert_{t=0^{-}}$ \\ \hline
				Integration & $\int_{0}^{t} x \left( \lambda \right) d\lambda$ & $\frac{1}{s} X(s)$ \\ \hline
				Multiply in Frequency, Convolution in Time & $x(t) * v(t)$ & $X(s)V(s)$ \\ \hline
				Initial Value Theorem & \multicolumn{2}{c|}{$x \left( 0^{+} \right) = \lim\limits_{s \rightarrow \infty} sX(s)$} \\ \hline
				Final Value Theorem & \multicolumn{2}{c|}{$\lim\limits_{t \rightarrow \infty} x(t) = \lim\limits_{s\rightarrow 0} sX(s)$} \\ \hline
				Relation to Fourier Transform & \multicolumn{2}{c|}{If $X(\omega)$ exists, then $X(s) = X(\omega)|_{\omega = \frac{s}{j}}$} \\ \hline
			\end{tabular}
		\end{table}
		\vspace{-5mm}
		
	\subsection*{Laplace Transform Pairs} \label{subsec:Laplace Transform Pairs}
		\begin{align*}
			\Lapl \lbrace x (t) \rbrace &= X(s) & \Lapl \lbrace \delta (t) \rbrace &= 1 & \Lapl \lbrace \delta \left( t-T_{0} \right) \rbrace &= e^{-stT_{0}} & \Lapl \lbrace \UnitStep (t) \rbrace &= \frac{1}{s} \\
			\Lapl \lbrace t \UnitStep (t) \rbrace &= \frac{1}{s^{2}} & \Lapl \lbrace t^{n}\UnitStep (t) \rbrace &= \frac{n!}{s^{n+1}} & \Lapl \lbrace \UnitStep \left( t-T_{0} \right) \rbrace &= \frac{e^{-sT_{0}}}{s} & \Lapl \lbrace e^{at} \UnitStep (t) \rbrace &= \frac{1}{\left( s-a \right)} \\
			\Lapl \lbrace t e^{at} \UnitStep (t) \rbrace &= \frac{1}{\left( s-a \right)^{2}} & \Lapl \lbrace t^{n} e^{at} \UnitStep (t) \rbrace &= \frac{n!}{\left( s-a \right)^{n+1}} & \Lapl \lbrace \cos \left( bt \right) \UnitStep (t) \rbrace &= \frac{s}{s^{2}-b^{2}} & \Lapl \lbrace \sin \left( bt \right) \UnitStep (t) \rbrace &= \frac{b}{s^{2}+b^{2}} \\
		\end{align*}
		\begin{align*}
			\Lapl \lbrace e^{-at} \cos \left( bt \right) \UnitStep (t) \rbrace &= \frac{s+a}{\left( s+a \right)^{2} + b^{2}} & \Lapl \lbrace e^{-at} \sin \left( bt \right) \UnitStep (t) \rbrace &= \frac{b}{\left( s+a \right)^{2} + b^{2}} \\
		\end{align*}
		\begin{equation*}
			\Lapl \lbrace r e^{-at} \cos \left( bt + \theta \right) \UnitStep (t) \rbrace =
				\begin{cases}
					a: & \frac{rs \cos \left( \theta \right) + ar \cos \left( \theta \right) - br \sin \left( \theta \right)}{s^{2} + 2as + \left( a^{2} + b^{2} \right)} \\
					b: & \frac{0.5 re^{j \theta}}{s+a-jb} + \frac{0.5 re^{-j \theta}}{s+a+jb} \\
					c: & \frac{As+B}{s^{2} + 2as + c}
						\begin{cases}
							r &=\sqrt{\frac{A^{2}c + B^{2} -2ABa}{c-a^{2}}} \\
							\theta &= \arctan \left( \frac{Aa-B}{A \sqrt{c-a^{2}}} \right)
						\end{cases} \\
				\end{cases}
		\end{equation*}
		\begin{equation*}
			\Lapl \lbrace e^{-at} \left( A \cos \left( bt \right) + \frac{B-Aa}{b} \sin \left( bt \right) \right) \UnitStep (t) \rbrace = \frac{As+B}{s^{2} + 2as + c} \\
			b = \sqrt{c-a^{2}}
		\end{equation*}